Tutorial/FormalVerification/StateMachine.lean
@@ -1,75 +1,89 @@
 /-
+The goal of this file is to show how formal verification can be used to prove the
+correctness of a simple state machine. We will define a workflow model and a `step`
+function that updates the state of the workflow based on certain events, and then
+prove that the `step` function preserves the safety of the workflow.
+
+For simplicity, our workflow will have two boolean fields: `started` and `completed`.
+The `started` field indicates whether the workflow has started or not, and the
+`completed` field indicates whether the workflow has completed or not.
+
+A workflow is considered `Safe` if it is not completed or if it is completed,
+then it must have been started.
+
+We then define a `step` function that takes a workflow and an event, and updates
+the state of the workflow based on the event.
+
+The main theorem we want to prove is that the `step` function preserves the
+safety of the workflow. In other words, we want to prove that:
+
+> If a workflow is `Safe` before an event, then it should still be `Safe` after
+> the event as well.
+-/
+
+/--
 A simple workflow can have three states:
 * Pending: the workflow has not started yet.
 * InProgress: the workflow has started but not completed yet.
 * Completed: the workflow has started and completed.
 
-The main invariant for a workflow is that it cannot be completed if it has not
-been started. In other words, the following invariant must hold:
-> If a workflow is completed, then it must have been started.
-
-We define a `Workflow` as a pair of two boolean values:
+We model the `Workflow` as a pair of two boolean values:
 * `started` which indicates whether the workflow has started or not.
 * `completed` which indicates whether the workflow has completed or not.
 
-It obeys the following truth table:
-| started | completed | Safe? |
-|---------|-----------|-------|
-| false   | false     | true  |
-| false   | true      | false |
-| true    | false     | true  |
-| true    | true      | true  |
-
-This is essentially the truth table for the implication `completed → started`,
-which is the invariant we want to use to label a workflow as `Safe`.
-
-> A workflow is `Safe` if it is not completed or if it is completed, then it
-> must have been started.
-
-In formal terms:
-> ∀ wf : Workflow, Safe wf ↔ (Completed wf → Started wf).
-
-An event that changes the state of the workflow can be either:
-* `start` which transitions the workflow from pending to in progress.
-* `complete` which transitions the workflow from in progress to completed.
-
-The `step` function takes a workflow and an event and returns the new workflow
-after applying the event.
--/
-
-/-
-A workflow keeps track of whether it has been started and completed. The main
-invariant is that a workflow cannot be completed if it has not been started.
+The model maps the states to the following values:
+| started | completed | State      |
+|---------|-----------|------------|
+| false   | false     | Pending    |
+| true    | false     | InProgress |
+| true    | true      | Completed  |
+| false   | true      | _invalid_  |
 -/
 structure Workflow where
   started   : Bool
   completed : Bool
 
-/-
+/--
 A workflow is `Safe` if it is not completed or if it is completed, then it must
 have been started.
+
+The safety of a workflow follows the truth table:
+| started | completed | Safe  |
+|---------|-----------|-------|
+| false   | false     | true  |
+| true    | false     | true  |
+| true    | true      | true  |
+| false   | true      | false |
+
+This is the truth table of the implication `completed → started`, which is the
+definition of the `Safe` invariant.
+
+In formal terms:
+> ∀ wf : Workflow, Safe wf ↔ (Completed wf → Started wf).
 -/
 def Safe (wf : Workflow) : Prop := wf.completed = true → wf.started = true
 
-/-
-An event changes the state of a given workflow.
+/--
+An event is used to change the state of a given workflow and can be either:
+* `start` which transitions the workflow from pending to in progress.
+* `complete` which transitions the workflow from in progress to completed.
 -/
 inductive Event where
   | start    : Event
   | complete : Event
 
-/-
-The `step` function update the state of the workflow based on the given event. It
+/--
+The `step` function updates the state of the workflow based on the given event. It
 follows the rules:
 * If the event is `start`, then the workflow is marked as started.
 * If the event is `complete` and the workflow has already been started, then it
   is marked as completed.
-* If the event is `complete` and the workflow has not been started, then the
+* If the event is `complete` and the workflow has *not* been started, then the
   workflow remains unchanged.
 -/
 def step : Workflow → Event → Workflow
-  | wf, Event.start => { wf with started := true }
-  | wf, Event.complete =>
+  | wf, .start => { wf with started := true }
+  | wf, .complete =>
     if wf.started then
       { wf with completed := true }
     else
@@ -77,19 +91,18 @@ def step : Workflow → Event → Workflow
 
 /-
 The main theorem we want to prove is that the `step` function preserves the
-`Safe` invariant.
-> If a workflow is `Safe` before an event, then it should still be `Safe` after
-> the event as well.
+`Safe` invariant meaning that if we start with a `Safe` workflow and apply any
+sequence of events using the `step` function, the resulting workflow will also
+be `Safe`.
 -/
 theorem step_preserves_safety (wf : Workflow) (e : Event) :
   Safe wf → Safe (step wf e) := by
   intro h_wf_safe      -- assumes that the workflow is safe before the event
   cases e with
   | start =>           -- if the event is `start`, then the new workflow is safe
-    unfold Safe at *
-    simp [step]
+    simp [Safe, step]
   | complete =>    -- if the event is `complete`, we consider the `started` state
-    unfold Safe at *
+    simp [Safe] at *
     cases h_started : wf.started
     . -- h_started = false → cannot be completed
       cases h_completed : wf.completed
@@ -107,7 +120,6 @@ theorem step_preserves_safety (wf : Workflow) (e : Event) :
       simp [step, h_started]
 
 /-
-With that, we have shown that the `step` function preserves the `Safe` invariant.
-This means that if we start with a `Safe` workflow and apply any sequence of
-events using the `step` function, the resulting workflow will also be `Safe`.
+This concludes our goal. We have successfully proved that the `step` function
+preserves the workflow's safety.
 -/
