Tutorial/FormalVerification/MapReduce.lean
@@ -1,32 +1,95 @@
-section Map
+/-
+The goal of this file is to show how formal verification can be used to prove code
+optimisation techniques, such as fusion and deforestation. We will define two
+common higher-order functions, `map` and `fold`, and then prove that they can be
+fused together to eliminate repeat traversals of the list.
+
+We want to prove two theorems:
+1. Fusion: A sequence of `map` operations can be fused into a single `map` with
+   a composed function.
+2. Deforestation: A `map` followed by a `fold` can be fused into a single `fold`
+   with a composed function.
+-/
+
+/--
+The `map` function takes a function `f : α → β` and a list of type `α`, and
+applies `f` to each element of the list, returning a new list of type `β`.
+
+The `map` function has the following invariants:
+* It preserves the length of the list: `length (map f xs) = length xs`.
+* It preserves the order of the elements: `map f (xs ++ ys) = map f xs ++ map f ys`.
+* It is composable: `map g (map f xs) = map (g ∘ f) xs`.
+
+The composability invariant is particularly important because it allows us to
+create complex transformations by composing simpler ones.
+-/
 def map (f : α → β) : List α → List β
   | [] => []
   | a::as => f a :: map f as
 
-#eval map (fun x => x + 1) [1, 2, 3]
+/--
+Fold (or reduce) is a common operation for aggregation. It takes a binary
+function `f : β → α → β`, an initial accumulator value `acc : β`, and a list of
+type `α`, and processes the list from left to right, applying `f` to the
+accumulator and each element of the list, returning a result result of type `β`.
 
-theorem fusion (f : α → β) (g : β → γ) : (map g) ∘ (map f) = map (g ∘ f) := by
-  funext xs
-  induction xs with
-  | nil => trivial
-  | cons a as h =>
-    simp? [map] at *
-    rw [h]
-end Map
+The `fold` function has the following invariants:
+* It is associative: `fold f acc (xs ++ ys) = fold f (fold f acc xs) ys`.
+* It has an identity element: if there exists an element `e` such that `f e x = x`
+  for all `x`, then `fold f e (x::xs) = fold f x xs`.
+* It is composable with `map`: `fold f acc (map g xs) = fold (λa ↦ (f a) ∘ g) acc xs`.
 
-section Reduce
+The composability with `map` invariant is crucial for deforestation, as it allows
+us to fuse `map` and `fold` together, eliminating intermediate lists and reducing
+the number of traversals of the list.
+-/
 def fold (f : β → α → β) (acc : β) : List α → β
   | [] => acc
   | x :: xs => fold f (f acc x) xs
 
+-- Let's see some examples.
+#eval map (fun x => x + 1) [1, 2, 3]
 #eval fold (fun acc x => acc + x) 0 [1, 2, 3]
 
-theorem deforastation (f : α → β) (g : γ → β → γ) (acc : γ) :
-  (fold g acc) ∘ (map f) = fold (λa ↦ (g a) ∘ f) acc := by
-  funext xs
-  induction xs generalizing acc with
-  | nil => trivial
-  | cons a as h =>
-    simp? [map, fold] at *
-    rw [h]
-end Reduce
+/--
+Two functions `f : α → β` and `g : β → γ` are composable if they don't have side
+effects.
+
+If `f` and `g` are composable, then mapping `f` over a list `xs : List α` and
+then mapping `g` over the result is the same as mapping the composition `g ∘ f`
+over `xs`.
+-/
+theorem fusion (f : α → β) (g : β → γ) (xs : List α) :
+  map g (map f xs) = map (g ∘ f) xs := by
+  induction xs with
+  | nil => trivial     -- mapping over an empty list must return an empty list
+  | cons a as ih =>    -- ih : induction hypothesis for the tail of the list
+     simp [map] at *
+     rw [ih]
+
+/--
+Two functions `f : α → β` and `g : γ → β → γ` are composable if they don't have
+side effects.
+
+If `f : α → β` and `g : γ → β → γ` are composable functions, given an initial
+value `acc : γ` and a list `xs : List α`, folding `g` over the result of mapping
+`f` is the same as folding a function `λa.λx. g a (f x)` over `xs` with the same
+initial value `acc`.
+-/
+theorem deforastation (f : α → β) (g : γ → β → γ) (acc : γ) (xs : List α) :
+  fold g acc (map f xs) = fold (fun a x => g a (f x)) acc xs := by
+  induction xs generalizing acc with  -- acc can be results from previous iterations
+  | nil => trivial   -- operations over an empty list must return the initial value
+  | cons a as ih =>  -- ih : induction hypothesis for the tail of the list
+     simp [map, fold] at *
+     rw [ih]
+
+/-
+This concludes our goal. We have successfully proved that mapping and folding
+composable functions can be merged into a single traversal operation.
+
+Fusion and deforestation are two of the reasons that make iterators so powerful.
+They allow us to express complex transformations by composing simple ones, while
+also allowing the compiler to optimize the code by eliminating intermediate data
+structures and reducing the number of traversals of the list.
+-/
